language/move-model/src/well_known.rs
@@ -7,8 +7,8 @@
 //! This currently only contains those declarations used somewhere, not all well-known
 //! declarations. It can be extended on the go.
 
-pub const VECTOR_BORROW_MUT: &str = "vector::borrow_mut";
-pub const EVENT_EMIT_EVENT: &str = "event::emit_event";
+pub const VECTOR_BORROW_MUT: &str = "Vector::borrow_mut";
+pub const EVENT_EMIT_EVENT: &str = "Event::emit_event";
 
 pub const TYPE_NAME_MOVE: &str = "type_info::type_name";
 pub const TYPE_NAME_SPEC: &str = "type_info::$type_name";
