language/move-prover/boogie-backend/src/prelude/native.bpl
@@ -74,27 +74,27 @@ function {:inline} $EmptyVec{{S}}(): Vec ({{T}}) {
     EmptyVec()
 }
 
-procedure {:inline 1} $1_vector_empty{{S}}() returns (v: Vec ({{T}})) {
+procedure {:inline 1} $1_Vector_empty{{S}}() returns (v: Vec ({{T}})) {
     v := EmptyVec();
 }
 
-function {:inline} $1_vector_$empty{{S}}(): Vec ({{T}}) {
+function {:inline} $1_Vector_$empty{{S}}(): Vec ({{T}}) {
     EmptyVec()
 }
 
-procedure {:inline 1} $1_vector_is_empty{{S}}(v: Vec ({{T}})) returns (b: bool) {
+procedure {:inline 1} $1_Vector_is_empty{{S}}(v: Vec ({{T}})) returns (b: bool) {
     b := IsEmptyVec(v);
 }
 
-procedure {:inline 1} $1_vector_push_back{{S}}(m: $Mutation (Vec ({{T}})), val: {{T}}) returns (m': $Mutation (Vec ({{T}}))) {
+procedure {:inline 1} $1_Vector_push_back{{S}}(m: $Mutation (Vec ({{T}})), val: {{T}}) returns (m': $Mutation (Vec ({{T}}))) {
     m' := $UpdateMutation(m, ExtendVec($Dereference(m), val));
 }
 
-function {:inline} $1_vector_$push_back{{S}}(v: Vec ({{T}}), val: {{T}}): Vec ({{T}}) {
+function {:inline} $1_Vector_$push_back{{S}}(v: Vec ({{T}}), val: {{T}}): Vec ({{T}}) {
     ExtendVec(v, val)
 }
 
-procedure {:inline 1} $1_vector_pop_back{{S}}(m: $Mutation (Vec ({{T}}))) returns (e: {{T}}, m': $Mutation (Vec ({{T}}))) {
+procedure {:inline 1} $1_Vector_pop_back{{S}}(m: $Mutation (Vec ({{T}}))) returns (e: {{T}}, m': $Mutation (Vec ({{T}}))) {
     var v: Vec ({{T}});
     var len: int;
     v := $Dereference(m);
@@ -107,23 +107,23 @@ procedure {:inline 1} $1_vector_pop_back{{S}}(m: $Mutation (Vec ({{T}}))) return
     m' := $UpdateMutation(m, RemoveVec(v));
 }
 
-procedure {:inline 1} $1_vector_append{{S}}(m: $Mutation (Vec ({{T}})), other: Vec ({{T}})) returns (m': $Mutation (Vec ({{T}}))) {
+procedure {:inline 1} $1_Vector_append{{S}}(m: $Mutation (Vec ({{T}})), other: Vec ({{T}})) returns (m': $Mutation (Vec ({{T}}))) {
     m' := $UpdateMutation(m, ConcatVec($Dereference(m), other));
 }
 
-procedure {:inline 1} $1_vector_reverse{{S}}(m: $Mutation (Vec ({{T}}))) returns (m': $Mutation (Vec ({{T}}))) {
+procedure {:inline 1} $1_Vector_reverse{{S}}(m: $Mutation (Vec ({{T}}))) returns (m': $Mutation (Vec ({{T}}))) {
     m' := $UpdateMutation(m, ReverseVec($Dereference(m)));
 }
 
-procedure {:inline 1} $1_vector_length{{S}}(v: Vec ({{T}})) returns (l: int) {
+procedure {:inline 1} $1_Vector_length{{S}}(v: Vec ({{T}})) returns (l: int) {
     l := LenVec(v);
 }
 
-function {:inline} $1_vector_$length{{S}}(v: Vec ({{T}})): int {
+function {:inline} $1_Vector_$length{{S}}(v: Vec ({{T}})): int {
     LenVec(v)
 }
 
-procedure {:inline 1} $1_vector_borrow{{S}}(v: Vec ({{T}}), i: int) returns (dst: {{T}}) {
+procedure {:inline 1} $1_Vector_borrow{{S}}(v: Vec ({{T}}), i: int) returns (dst: {{T}}) {
     if (!InRangeVec(v, i)) {
         call $ExecFailureAbort();
         return;
@@ -131,11 +131,11 @@ procedure {:inline 1} $1_vector_borrow{{S}}(v: Vec ({{T}}), i: int) returns (dst
     dst := ReadVec(v, i);
 }
 
-function {:inline} $1_vector_$borrow{{S}}(v: Vec ({{T}}), i: int): {{T}} {
+function {:inline} $1_Vector_$borrow{{S}}(v: Vec ({{T}}), i: int): {{T}} {
     ReadVec(v, i)
 }
 
-procedure {:inline 1} $1_vector_borrow_mut{{S}}(m: $Mutation (Vec ({{T}})), index: int)
+procedure {:inline 1} $1_Vector_borrow_mut{{S}}(m: $Mutation (Vec ({{T}})), index: int)
 returns (dst: $Mutation ({{T}}), m': $Mutation (Vec ({{T}})))
 {
     var v: Vec ({{T}});
@@ -148,17 +148,17 @@ returns (dst: $Mutation ({{T}}), m': $Mutation (Vec ({{T}})))
     m' := m;
 }
 
-function {:inline} $1_vector_$borrow_mut{{S}}(v: Vec ({{T}}), i: int): {{T}} {
+function {:inline} $1_Vector_$borrow_mut{{S}}(v: Vec ({{T}}), i: int): {{T}} {
     ReadVec(v, i)
 }
 
-procedure {:inline 1} $1_vector_destroy_empty{{S}}(v: Vec ({{T}})) {
+procedure {:inline 1} $1_Vector_destroy_empty{{S}}(v: Vec ({{T}})) {
     if (!IsEmptyVec(v)) {
       call $ExecFailureAbort();
     }
 }
 
-procedure {:inline 1} $1_vector_swap{{S}}(m: $Mutation (Vec ({{T}})), i: int, j: int) returns (m': $Mutation (Vec ({{T}})))
+procedure {:inline 1} $1_Vector_swap{{S}}(m: $Mutation (Vec ({{T}})), i: int, j: int) returns (m': $Mutation (Vec ({{T}})))
 {
     var v: Vec ({{T}});
     v := $Dereference(m);
@@ -169,11 +169,11 @@ procedure {:inline 1} $1_vector_swap{{S}}(m: $Mutation (Vec ({{T}})), i: int, j:
     m' := $UpdateMutation(m, SwapVec(v, i, j));
 }
 
-function {:inline} $1_vector_$swap{{S}}(v: Vec ({{T}}), i: int, j: int): Vec ({{T}}) {
+function {:inline} $1_Vector_$swap{{S}}(v: Vec ({{T}}), i: int, j: int): Vec ({{T}}) {
     SwapVec(v, i, j)
 }
 
-procedure {:inline 1} $1_vector_remove{{S}}(m: $Mutation (Vec ({{T}})), i: int) returns (e: {{T}}, m': $Mutation (Vec ({{T}})))
+procedure {:inline 1} $1_Vector_remove{{S}}(m: $Mutation (Vec ({{T}})), i: int) returns (e: {{T}}, m': $Mutation (Vec ({{T}})))
 {
     var v: Vec ({{T}});
 
@@ -187,7 +187,7 @@ procedure {:inline 1} $1_vector_remove{{S}}(m: $Mutation (Vec ({{T}})), i: int) 
     m' := $UpdateMutation(m, RemoveAtVec(v, i));
 }
 
-procedure {:inline 1} $1_vector_swap_remove{{S}}(m: $Mutation (Vec ({{T}})), i: int) returns (e: {{T}}, m': $Mutation (Vec ({{T}})))
+procedure {:inline 1} $1_Vector_swap_remove{{S}}(m: $Mutation (Vec ({{T}})), i: int) returns (e: {{T}}, m': $Mutation (Vec ({{T}})))
 {
     var len: int;
     var v: Vec ({{T}});
@@ -202,12 +202,12 @@ procedure {:inline 1} $1_vector_swap_remove{{S}}(m: $Mutation (Vec ({{T}})), i: 
     m' := $UpdateMutation(m, RemoveVec(SwapVec(v, i, len-1)));
 }
 
-procedure {:inline 1} $1_vector_contains{{S}}(v: Vec ({{T}}), e: {{T}}) returns (res: bool)  {
+procedure {:inline 1} $1_Vector_contains{{S}}(v: Vec ({{T}}), e: {{T}}) returns (res: bool)  {
     res := $ContainsVec{{S}}(v, e);
 }
 
 procedure {:inline 1}
-$1_vector_index_of{{S}}(v: Vec ({{T}}), e: {{T}}) returns (res1: bool, res2: int) {
+$1_Vector_index_of{{S}}(v: Vec ({{T}}), e: {{T}}) returns (res1: bool, res2: int) {
     res2 := $IndexOfVec{{S}}(v, e);
     if (res2 >= 0) {
         res1 := true;
@@ -439,34 +439,34 @@ function {:inline} {{impl.fun_spec_get}}{{S}}(t: {{Self}}, k: {{K}}): {{V}} {
 // Serialize is modeled as an uninterpreted function, with an additional
 // axiom to say it's an injection.
 
-function $1_bcs_serialize{{S}}(v: {{T}}): Vec int;
+function $1_BCS_serialize{{S}}(v: {{T}}): Vec int;
 
-axiom (forall v1, v2: {{T}} :: {$1_bcs_serialize{{S}}(v1), $1_bcs_serialize{{S}}(v2)}
-   $IsEqual{{S}}(v1, v2) <==> $IsEqual'vec'u8''($1_bcs_serialize{{S}}(v1), $1_bcs_serialize{{S}}(v2)));
+axiom (forall v1, v2: {{T}} :: {$1_BCS_serialize{{S}}(v1), $1_BCS_serialize{{S}}(v2)}
+   $IsEqual{{S}}(v1, v2) <==> $IsEqual'vec'u8''($1_BCS_serialize{{S}}(v1), $1_BCS_serialize{{S}}(v2)));
 
 // This says that serialize returns a non-empty vec<u8>
 {% if options.serialize_bound == 0 %}
-axiom (forall v: {{T}} :: {$1_bcs_serialize{{S}}(v)}
-     ( var r := $1_bcs_serialize{{S}}(v); $IsValid'vec'u8''(r) && LenVec(r) > 0 ));
+axiom (forall v: {{T}} :: {$1_BCS_serialize{{S}}(v)}
+     ( var r := $1_BCS_serialize{{S}}(v); $IsValid'vec'u8''(r) && LenVec(r) > 0 ));
 {% else %}
-axiom (forall v: {{T}} :: {$1_bcs_serialize{{S}}(v)}
-     ( var r := $1_bcs_serialize{{S}}(v); $IsValid'vec'u8''(r) && LenVec(r) > 0 &&
+axiom (forall v: {{T}} :: {$1_BCS_serialize{{S}}(v)}
+     ( var r := $1_BCS_serialize{{S}}(v); $IsValid'vec'u8''(r) && LenVec(r) > 0 &&
                             LenVec(r) <= {{options.serialize_bound}} ));
 {% endif %}
 
-procedure $1_bcs_to_bytes{{S}}(v: {{T}}) returns (res: Vec int);
-ensures res == $1_bcs_serialize{{S}}(v);
+procedure $1_BCS_to_bytes{{S}}(v: {{T}}) returns (res: Vec int);
+ensures res == $1_BCS_serialize{{S}}(v);
 
-function {:inline} $1_bcs_$to_bytes{{S}}(v: {{T}}): Vec int {
-    $1_bcs_serialize{{S}}(v)
+function {:inline} $1_BCS_$to_bytes{{S}}(v: {{T}}): Vec int {
+    $1_BCS_serialize{{S}}(v)
 }
 
 {% if S == "'address'" -%}
 // Serialized addresses should have the same length.
 const $serialized_address_len: int;
 // Serialized addresses should have the same length
-axiom (forall v: int :: {$1_bcs_serialize'address'(v)}
-     ( var r := $1_bcs_serialize'address'(v); LenVec(r) == $serialized_address_len));
+axiom (forall v: int :: {$1_BCS_serialize'address'(v)}
+     ( var r := $1_BCS_serialize'address'(v); LenVec(r) == $serialized_address_len));
 {% endif %}
 {% endmacro hash_module %}
 
@@ -480,13 +480,13 @@ axiom (forall v: int :: {$1_bcs_serialize'address'(v)}
 {%- set T = instance.name -%}
 
 // Map type specific handle to universal one.
-type $1_event_EventHandle{{S}} = $1_event_EventHandle;
+type $1_Event_EventHandle{{S}} = $1_Event_EventHandle;
 
-function {:inline} $IsEqual'$1_event_EventHandle{{S}}'(a: $1_event_EventHandle{{S}}, b: $1_event_EventHandle{{S}}): bool {
+function {:inline} $IsEqual'$1_Event_EventHandle{{S}}'(a: $1_Event_EventHandle{{S}}, b: $1_Event_EventHandle{{S}}): bool {
     a == b
 }
 
-function $IsValid'$1_event_EventHandle{{S}}'(h: $1_event_EventHandle{{S}}): bool {
+function $IsValid'$1_Event_EventHandle{{S}}'(h: $1_Event_EventHandle{{S}}): bool {
     true
 }
 
@@ -498,45 +498,45 @@ axiom (forall v1, v2: {{T}} :: {$ToEventRep{{S}}(v1), $ToEventRep{{S}}(v2)}
 // Creates a new event handle. This ensures each time it is called that a unique new abstract event handler is
 // returned.
 // TODO: we should check (and abort with the right code) if no generator exists for the signer.
-procedure {:inline 1} $1_event_new_event_handle{{S}}(signer: $signer) returns (res: $1_event_EventHandle{{S}}) {
-    assume $1_event_EventHandles[res] == false;
-    $1_event_EventHandles := $1_event_EventHandles[res := true];
+procedure {:inline 1} $1_Event_new_event_handle{{S}}(signer: $signer) returns (res: $1_Event_EventHandle{{S}}) {
+    assume $1_Event_EventHandles[res] == false;
+    $1_Event_EventHandles := $1_Event_EventHandles[res := true];
 }
 
 // This boogie procedure is the model of `emit_event`. This model abstracts away the `counter` behavior, thus not
 // mutating (or increasing) `counter`.
-procedure {:inline 1} $1_event_emit_event{{S}}(handle_mut: $Mutation $1_event_EventHandle{{S}}, msg: {{T}})
-returns (res: $Mutation $1_event_EventHandle{{S}}) {
-    var handle: $1_event_EventHandle{{S}};
+procedure {:inline 1} $1_Event_emit_event{{S}}(handle_mut: $Mutation $1_Event_EventHandle{{S}}, msg: {{T}})
+returns (res: $Mutation $1_Event_EventHandle{{S}}) {
+    var handle: $1_Event_EventHandle{{S}};
     handle := $Dereference(handle_mut);
     $es := $ExtendEventStore{{S}}($es, handle, msg);
     res := handle_mut;
 }
 
-procedure {:inline 1} $1_event_guid{{S}}(handle_ref: $1_event_EventHandle{{S}})
+procedure {:inline 1} $1_Event_guid{{S}}(handle_ref: $1_Event_EventHandle{{S}})
 returns (res: int) {
     // TODO: temporarily mocked. The return type needs to be fixed.
     res := 0;
 }
 
-procedure {:inline 1} $1_event_counter{{S}}(handle_ref: $1_event_EventHandle{{S}})
+procedure {:inline 1} $1_Event_counter{{S}}(handle_ref: $1_Event_EventHandle{{S}})
 returns (res: int) {
     // TODO: temporarily mocked.
     res := 0;
 }
 
-procedure {:inline 1} $1_event_destroy_handle{{S}}(handle: $1_event_EventHandle{{S}}) {
+procedure {:inline 1} $1_Event_destroy_handle{{S}}(handle: $1_Event_EventHandle{{S}}) {
 }
 
 function {:inline} $ExtendEventStore{{S}}(
-        es: $EventStore, handle: $1_event_EventHandle{{S}}, msg: {{T}}): $EventStore {
+        es: $EventStore, handle: $1_Event_EventHandle{{S}}, msg: {{T}}): $EventStore {
     (var stream := streams#$EventStore(es)[handle];
     (var stream_new := ExtendMultiset(stream, $ToEventRep{{S}}(msg));
     $EventStore(counter#$EventStore(es)+1, streams#$EventStore(es)[handle := stream_new])))
 }
 
 function {:inline} $CondExtendEventStore{{S}}(
-        es: $EventStore, handle: $1_event_EventHandle{{S}}, msg: {{T}}, cond: bool): $EventStore {
+        es: $EventStore, handle: $1_Event_EventHandle{{S}}, msg: {{T}}, cond: bool): $EventStore {
     if cond then
         $ExtendEventStore{{S}}(es, handle, msg)
     else
